theories/examples/enclaves/mutual_attestation_A_spec.v
@@ -1,0 +1,58 @@
+From iris.proofmode Require Import proofmode.
+From cap_machine Require Import rules logrel fundamental.
+From cap_machine Require Import proofmode.
+From cap_machine Require Import mutual_attestation_code.
+
+Section mutual_attest_A.
+  Context {Σ:gFunctors} {ceriseg:ceriseG Σ} {sealsg : sealStoreG Σ}
+    {nainv: logrel_na_invs Σ} `{MP: MachineParameters}.
+  Context {MA: MutualAttestation}.
+
+  Ltac iHide0 irisH coqH :=
+    let coqH := fresh coqH in
+    match goal with
+    | h: _ |- context [ environments.Esnoc _ (INamed irisH) ?prop ] =>
+        set (coqH := prop)
+    end.
+
+  Tactic Notation "iHide" constr(irisH) "as" ident(coqH) :=
+    iHide0 irisH coqH.
+
+
+  (* -------------------------------------------------- *)
+  (* ------------------ ENCLAVE A---------------------- *)
+  (* -------------------------------------------------- *)
+
+  Lemma mutual_attest_A_contract
+    v b' e' a' v'
+    enclave_data ot :
+    let e := (length mutual_attest_enclave_A_code + 1)%Z in
+    (ot + 2)%f = Some (ot ^+ 2)%f ->
+    (b' < e')%a ->
+    (ma_addr_A + e)%a =
+    Some (ma_addr_A ^+ e)%a ->
+    custom_enclave_inv ma_enclaves_map
+    ∗ na_inv logrel_nais (custom_enclaveN.@hash_mutual_attest_A)
+        ([[ma_addr_A,(ma_addr_A ^+ e)%a]]↦ₐ{v}
+           [[LCap RW b' e' a' v' :: mutual_attest_enclave_A_code]]
+         ∗ [[b',e']]↦ₐ{v'}[[LSealRange (true, true) ot (ot ^+ 2)%f ot :: enclave_data]])
+    ∗ seal_pred (ot ^+ 1)%f sealed_enclaveA
+      -∗ interp (LCap E ma_addr_A
+                   (ma_addr_A ^+ e)%a
+                   (ma_addr_A ^+ 1)%a v).
+  Proof.
+    intro e ; subst e.
+    iIntros (Hot Hb' He) "#(Henclaves_inv & Hma_inv & HPsign)".
+    rewrite fixpoint_interp1_eq /=.
+    iIntros (lregs); iNext ; iModIntro.
+    iIntros "([%Hfullmap #Hinterp_map] & Hrmap & Hna)".
+    rewrite /interp_conf.
+    iMod (na_inv_acc with "Hma_inv Hna") as "(>[Hma_code Hma_data]  & Hna & Hclose)"; [solve_ndisj ..|].
+    rewrite /registers_mapsto.
+    iExtract "Hrmap" PC as "HPC".
+    remember ma_addr_A as pc_b in |- * at 7.
+    (* remember (ma_addr_A ^+ (91%nat + 1))%a as pc_e in |- * at 4. *)
+    (* assert (SubBounds pc_b pc_e ma_addr_A (ma_addr_A ^+ (91%nat + 1))%a) by (subst; solve_addr). *)
+  Admitted.
+
+End mutual_attest_A.
