theories/examples/enclaves/mutual_attestation_code.v
@@ -1,0 +1,410 @@
+From iris.proofmode Require Import proofmode.
+From cap_machine Require Import logrel proofmode.
+
+(* -------------------------------------- *)
+(* --------------- AXIOMS --------------- *)
+(* -------------------------------------- *)
+
+Axiom hash_concat_app : forall `{MachineParameters} {A : Type} (la la' : list A),
+  hash (la++la') = hash_concat (hash la) (hash la').
+Axiom hash_concat_assoc : forall `{MachineParameters}, Assoc eq hash_concat.
+Instance hash_concat_Assoc `{MachineParameters} : Assoc eq hash_concat := hash_concat_assoc.
+
+Class MutualAttestation := {
+    ma_addr_A : Addr;
+    ma_addr_B : Addr
+  }.
+
+Section mutual_attest_example.
+  Context {Σ:gFunctors} {ceriseg:ceriseG Σ} {sealsg : sealStoreG Σ}
+    {nainv: logrel_na_invs Σ} `{MP: MachineParameters}.
+  Context {MA: MutualAttestation}.
+
+  (* --------------------------------------- *)
+  (* ------- MUTUAL ATTEST ENCLAVE A ------- *)
+  (* --------------------------------------- *)
+
+  (* Expects:
+     - r_t0 contains return pointer to adv
+   *)
+  Definition mutual_attest_enclave_A_code_pre : list LWord :=
+    encodeInstrsLW [
+
+
+      (* SEND {(O,a,a+1,42)}_signed_A ; with a%2=0 *)
+
+      (* fetch data_cap *)
+      Mov r_t5 PC;          (* r5 := (RX, pc_b, pc_e, pc_a) *)
+      GetA r_t1 r_t5;       (* r1 := pc_a *)
+      GetB r_t2 r_t5;       (* r2 := pc_b *)
+      Sub r_t1 r_t2 r_t1;   (* r1 := pc_b - pc_a *)
+      Lea r_t5 r_t1;        (* r5 := (RX, pc_b, pc_e, pc_b) *)
+      Load r_t1 r_t5;       (* r1 := (RW, data_b, data_e, data_a) *)
+
+      (* fetch sign_key *)
+      GetA r_t2 r_t1;       (* r2 := data_a *)
+      GetB r_t3 r_t1;       (* r3 := data_b *)
+      Sub r_t2 r_t3 r_t2;   (* r2 := data_b - data_a *)
+      Lea r_t1 r_t2;        (* r1 := (RW, data_b, data_e, data_b) *)
+      Load r_t6 r_t1;       (* r6 := [SU, σ, σ+2, σ] *)
+
+
+      Mov r_t4 r_t1;      (* r4 := (RW, data_b, data_e, data_b) *)
+      GetB r_t2 r_t1;     (* r2 := data_b *)
+      Add r_t3 r_t2 1;    (* r3 := data_b + 1 *)
+      Subseg r_t1 r_t2 r_t3; (* r1 := (RW, data_b, data_b+1, data_b) *)
+      Add r_t5 r_t3 1;    (* r5 := data_b + 2 *)
+      Subseg r_t4 r_t3 r_t5; (* r4 := (RW, data_b+1, data_b+2, data_b) *)
+
+      (* fetch sign key *)
+
+
+
+
+
+
+      (* fetch ?malloc *)
+      (* hash ?malloc *)
+      (* if #?malloc =! #malloc_entry_point --> fail *)
+
+      (* malloc a buffer b of size 3:
+         will be used to communicate
+      *)
+
+      (* let idA := hash PC[1::-] *)
+      (* let idT := data[0-1] *)
+
+      (* if idA != idT, then fail *)
+
+      (* hash idT *)
+
+      (* let mbA := base(b) % 3 *)
+      (* if mbA == 0,
+         then we can use
+         + mbA[0] for #idT
+         + mbA[1] for 42    // attestation of A for B
+         + mbA[2] for 1     // attestation of A for main
+       *)
+      (* if mbA == 1,
+         then we can use
+         + mbA[0] for 1     // attestation of A for main
+         + mbA[1] for #idT
+         + mbA[2] for 42    // attestation of A for B
+       *)
+      (* if mbA == 2,
+         then we can use
+         + mbA[0] for 42    // attestation of A for B
+         + mbA[1] for 1     // attestation of A for main
+         + mbA[2] for #idT
+       *)
+
+      (* fetch sign key *)
+      (* signs { mbA[#idT] }_signed_A *)
+      (* signs { mbA[w42] }_signed_A *)
+
+      (* call ENCLAVE B with
+        r_t30 := return pointer;
+        r_t1  := { mbA[#idT] }_signed_A;
+        r_t2  := { mbA[w42] }_signed_A;
+        r_t3  := pub_sign_key_A;
+      *)
+
+      (* ---- we only arrive here if B has successfully attested A ---- *)
+      (* receives:
+        r_t1  := { mbB[#idT] }_signed_B;
+        r_t2  := { mbB[w43] }_signed_B;
+        r_t3  := pub_sign_key_B;
+      *)
+
+      (* ATTEST B *)
+      (* TODO @June: how do I attest
+         the value returned by B
+      *)
+      (* if mbA[#idT] != mbB[#idT], then fail *)
+
+      (* CHECK ATTESTS B *)
+      (* get idT(B) in r_t2 *)
+      (* get hash(idT) in r_t3 *)
+      (* get hash_concat(idT(B),idT) in r_t3 *)
+
+      (* compare identity(r_t1) == r_t3 *)
+
+      (* assert unsealed( {43}_signed_B ) = 43 *)
+
+      Jmp r_t0
+      (* REST OF CODE OF A *)
+    ].
+
+
+
+  (* --------------------------------------- *)
+  (* ------- MUTUAL ATTEST ENCLAVE B ------- *)
+  (* --------------------------------------- *)
+
+
+  Definition mutual_attest_enclave_B_mod_encoding : list LWord :=
+    encodeInstrsLW [
+        (* if x%2 = 0 then mb=[42;1] else  mb=[1;42] *)
+        Mod r_t3 r_t2 2;
+        Mov r_t5 PC;
+        Lea r_t5 9;
+        Jnz r_t5 r_t3;
+
+        (* case x%2 == 0 *)
+        Sub r_t3 43 r_t2;
+        Lea r_t1 r_t3; (*  r1 :=  (RW, data_b, data_b+1, 42) *)
+        Sub r_t3 1 r_t2;
+        Lea r_t4 r_t3; (*  r4 :=  (RW, data_b+1, data_b+2, 1) *)
+        Lea r_t5 4;
+        Jmp r_t5;
+
+        (* case x%2 == 1 *)
+        Sub r_t3 1 r_t2;
+        Lea r_t1 r_t3; (*  r1 :=  (RW, data_b, data_b+1, 1) *)
+        Sub r_t3 43 r_t2;
+        Lea r_t4 r_t3 (*  r4 :=  (RW, data_b+1, data_b+2, 42) *)
+      ].
+
+  (* Expects:
+     - r_t0 contains return pointer to caller
+     - r_t1 contains entry point to ENCLAVE B, not attested yet
+   *)
+  Definition mutual_attest_enclave_B_code_pre : list LWord :=
+    let size_idT : Z := 2 in
+    let offset_idA : Z := 0 in
+    let offset_idB : Z := 1 in
+    encodeInstrsLW [
+      (* CODE INITIALISATION ENCLAVE B *)
+
+      (* receives:
+         r_t1 := {42}_signed_A;
+         r_t2 := pub_sign_key_A;
+      *)
+
+      (* CHECK ATTESTS A *)
+      (* get idT(A) in r_t3 *)
+
+      Mov r_t4 PC;                (* r4 := (RX, pc_b, pc_e, pc_a) *)
+      GetA r_t5 r_t4;             (* r5 := pc_a *)
+      GetE r_t6 r_t4;             (* r6 := pc_e *)
+      Sub r_t5 r_t6 r_t5;         (* r5 := pc_e - pc_a *)
+      Lea r_t4 r_t5;              (* r4 := (RX, pc_b, pc_e, pc_e) *)
+      Lea r_t4 (-size_idT)%Z;     (* r4 := (RX, pc_b, pc_e, a_idT) *)
+
+      Mov r_t3 r_t4;              (* r3 := (RX, pc_b, pc_e, a_idT) *)
+      Lea r_t3 offset_idA;        (* r3 := (RX, pc_b, pc_e, a_idT(A)) *)
+      Load r_t3 r_t3;             (* r3 := idT(A) *)
+
+      (* get hash(idT) in r_t4 *)
+      GetA r_t5 r_t4;             (* r5 := a_idT *)
+      Subseg r_t4 r_t5 r_t6;      (* r4 := (RX, a_idT pc_e, a_idT) *)
+      Hash r_t4 r_t4;             (* r4 := #[a_idT;pc_E] *)
+
+      (* get hash_concat(idT(A),idT) in r_t3 *)
+      HashConcat r_t3 r_t3 r_t4;  (* r3 := idT(A) || #[a_idT;pc_E] *)
+
+      (* compare identity(r_t1) == r_t3 *)
+      GetOType r_t4 r_t1;         (* r4 := ?signed_A *)
+      Add r_t4 r_t4 1;            (* r5 := if is_sealed(r_t1) = false then 0 else not0 *)
+
+      (* if  is_sealed(r_t1) then continue else fail *)
+      Mov r_t5 PC;
+      Lea r_t5 4;
+      Jnz r_t5 r_t4;
+      Fail;
+
+      GetOType r_t5 r_t1;         (* r5 := ?signed_A *)
+      EStoreId r_t4 r_t5;         (* r4 := I_signed_A *)
+      Sub r_t3 r_t3 r_t4;         (* r3 := (idT(A) || #[a_idT;pc_E]) - ?signed_A*)
+
+      (* if ?signed_A != (idT(A) || #[a_idT;pc_E])
+         then Fail
+         else continue *)
+      Mov r_t5 PC;
+      Lea r_t5 5;
+      Jnz r_t5 r_t3;
+      Lea r_t5 1;
+      Jmp r_t5;
+      Fail;
+
+      UnSeal r_t1 r_t2 r_t1;      (* r1 := unsealed( {(RO,a, _, 42)}_signed_A ) *)
+      (* if (unsealed( {42}_signed_A ) != 42)
+         then Fail
+         else continue
+       *)
+
+      GetB r_t2 r_t1;             (* r2 := a *)
+      Mod r_t2 r_t2 2;            (* r2 := a%2 *)
+      (* if a%2 != 0 then Fail else continue *)
+      Mov r_t5 PC;
+      Lea r_t5 5;
+      Jnz r_t5 r_t2;
+      Lea r_t5 1;
+      Jmp r_t5;
+      Fail;
+
+      GetA r_t1 r_t1; (* r1 := ?42 *)
+      (* if ?42 != 42 then Fail else continue *)
+      Sub r_t1 r_t1 42;
+      Lea r_t5 6;
+      Jnz r_t5 r_t2;
+      Lea r_t5 1;
+      Jmp r_t5;
+      Fail;
+
+      (* fetch data_cap *)
+      GetA r_t1 r_t5;
+      GetB r_t2 r_t5;
+      Sub r_t1 r_t2 r_t1;
+      Lea r_t5 r_t1;
+      Load r_t1 r_t5;       (* r1 := (RW, data_b, data_e, data_a) *)
+
+      (* fetch sign_key *)
+      GetA r_t2 r_t1;
+      GetB r_t3 r_t1;      (* r3 := data_b *)
+      Sub r_t2 r_t3 r_t2;
+      Lea r_t1 r_t2;       (* r1 := (RW, data_b, data_e, data_b) *)
+      Load r_t6 r_t1;      (* r6 := [SU, σ, σ+2, σ] *)
+
+
+      Mov r_t4 r_t1;      (* r4 := (RW, data_b, data_e, data_b) *)
+      GetB r_t2 r_t1;     (* r2 := data_b *)
+      Add r_t3 r_t2 1;    (* r3 := data_b + 1 *)
+      Subseg r_t1 r_t2 r_t3; (* r1 := (RW, data_b, data_b+1, data_b) *)
+      Add r_t5 r_t3 1;    (* r5 := data_b + 2 *)
+      Subseg r_t4 r_t3 r_t5 (* r4 := (RW, data_b+1, data_b+2, data_b) *)
+      ]
+      ++ mutual_attest_enclave_B_mod_encoding
+      ++ encodeInstrsLW [
+      (* continue here  *)
+      Restrict r_t1 (encodePerm O);
+      Restrict r_t4 (encodePerm O);
+
+      (* sign x and sign x+1 *)
+      Lea r_t6 1;            (* r6 := (SU, σ+1, σ+2, σ+1) *)
+      Seal r_t1 r_t6 r_t1;
+      Seal r_t2 r_t6 r_t4;
+
+      GetA r_t3 r_t6;        (* r3 := σ+1 *)
+      Add r_t4 r_t3 1;       (* r4 := σ+2 *)
+      Subseg r_t6 r_t3 r_t4; (* r6 := (SU, σ+1, σ+2, σ+1) *)
+      Restrict r_t6 (encodeSealPerms (false,true));
+
+      (* clear regs and jmp to adv *)
+      Mov r_t3 r_t6;
+      Mov r_t4 0;
+      Mov r_t5 0;
+      Mov r_t6 0;
+      Jmp r_t0
+    ].
+
+  (* Enclave Identity Table --- pre-hashed code *)
+  Definition hash_mutual_attest_A_pre : Z :=
+    hash_concat (hash ma_addr_A) (hash mutual_attest_enclave_A_code_pre).
+  Definition hash_mutual_attest_B_pre : Z :=
+    hash_concat (hash ma_addr_B) (hash mutual_attest_enclave_B_code_pre).
+
+  Definition mutual_attest_eid_table : list LWord :=
+    [ LWInt hash_mutual_attest_A_pre ; LWInt hash_mutual_attest_B_pre].
+
+
+  (* Fully hashed enclaves --- machine hashed enclaves *)
+  Definition mutual_attest_enclave_A_code : list LWord :=
+   (mutual_attest_enclave_A_code_pre ++ mutual_attest_eid_table).
+  Definition mutual_attest_enclave_B_code : list LWord :=
+   (mutual_attest_enclave_B_code_pre ++ mutual_attest_eid_table).
+
+  Definition hash_mutual_attest_A : Z :=
+    hash_concat (hash ma_addr_A) (hash mutual_attest_enclave_A_code).
+  Definition hash_mutual_attest_B : Z :=
+    hash_concat (hash ma_addr_B) (hash mutual_attest_enclave_B_code).
+
+  Definition mutual_attest_enclave_A (enclave_data_cap : LWord) : list LWord :=
+    enclave_data_cap::mutual_attest_enclave_A_code ++ mutual_attest_eid_table.
+  Definition mutual_attest_enclave_B (enclave_data_cap : LWord) : list LWord :=
+    enclave_data_cap::mutual_attest_enclave_B_code  ++ mutual_attest_eid_table.
+
+
+
+  (* Sealed predicate for enclave A *)
+  Program Definition f42 : Addr := (finz.FinZ 42 eq_refl eq_refl).
+  Program Definition f1 : Addr := (finz.FinZ 1 eq_refl eq_refl).
+  Definition prot_sealed_A (a : Addr) : Addr :=
+    if (decide (a `mod` 2%nat = 0 )%Z) then f42 else f1.
+
+  Definition sealed_enclaveA : LWord → iProp Σ :=
+    λ w, (∃ (b e : Addr) v,
+             ⌜ w = LCap O b e (prot_sealed_A b) v ⌝)%I.
+  Definition sealed_enclaveA_ne : (leibnizO LWord) -n> (iPropO Σ) :=
+      λne (w : leibnizO LWord), sealed_enclaveA w%I.
+
+  Instance sealed_enclaveA_persistent (w : LWord) : Persistent (sealed_enclaveA w).
+  Proof. apply _. Qed.
+
+  Definition seal_pred_enclaveA (τ : OType) := seal_pred τ sealed_enclaveA.
+  Definition valid_sealed_enclaveA_cap (w : LWord) (τ : OType) := valid_sealed w τ sealed_enclaveA.
+  Lemma sealed_enclaveA_interp (lw : LWord) : sealed_enclaveA lw -∗ fixpoint interp1 lw.
+  Proof.
+    iIntros "Hsealed".
+    iDestruct "Hsealed" as (b e v) "->".
+    by rewrite fixpoint_interp1_eq /=.
+  Qed.
+
+
+
+
+  (* Sealed predicate for enclave B *)
+  Program Definition f43 : Addr := (finz.FinZ 43 eq_refl eq_refl).
+  Definition prot_sealed_B (a : Addr) : Addr :=
+    if (decide (a `mod` 2%nat = 0 )%Z) then f43 else f1.
+
+  Definition sealed_enclaveB : LWord → iProp Σ :=
+    λ w, (∃ (b e : Addr) v,
+             ⌜ w = LCap O b e (prot_sealed_B b) v ⌝)%I.
+  Definition sealed_enclaveB_ne : (leibnizO LWord) -n> (iPropO Σ) :=
+      λne (w : leibnizO LWord), sealed_enclaveB w%I.
+
+  Instance sealed_enclaveB_persistent (w : LWord) : Persistent (sealed_enclaveB w).
+  Proof. apply _. Qed.
+
+  Definition seal_pred_enclaveB (τ : OType) := seal_pred τ sealed_enclaveB.
+  Definition valid_sealed_enclaveB_cap (w : LWord) (τ : OType) := valid_sealed w τ sealed_enclaveB.
+  Lemma sealed_enclaveB_interp (lw : LWord) : sealed_enclaveB lw -∗ fixpoint interp1 lw.
+  Proof.
+    iIntros "Hsealed".
+    iDestruct "Hsealed" as (b e v) "->".
+    by rewrite fixpoint_interp1_eq /=.
+  Qed.
+
+
+
+
+  (* Trusted Compute Custom Predicates *)
+  Definition mutual_attest_enclave_A_pred : CustomEnclave :=
+    @MkCustomEnclave Σ
+      mutual_attest_enclave_A_code
+      ma_addr_A
+      (λ w, False%I)
+      sealed_enclaveA.
+  Definition mutual_attest_enclave_B_pred : CustomEnclave :=
+    @MkCustomEnclave Σ
+      mutual_attest_enclave_B_code
+      ma_addr_B
+      (λ w, False%I)
+      sealed_enclaveB.
+
+  Definition ma_enclaves_map : custom_enclaves_map :=
+   {[ hash_mutual_attest_A := mutual_attest_enclave_A_pred;
+      hash_mutual_attest_B := mutual_attest_enclave_B_pred
+   ]}.
+
+  Lemma wf_ma_enclaves_map :
+    custom_enclaves_map_wf ma_enclaves_map.
+  Proof.
+    rewrite /custom_enclaves_map_wf /ma_enclaves_map.
+    apply (map_Forall_insert_2 (λ (I : Z) (ce : CustomEnclave), _)).
+    - by rewrite /hash_mutual_attest_A /=.
+    - by rewrite map_Forall_singleton /hash_mutual_attest_B /=.
+  Qed.
+
+End mutual_attest_example.
