theories/examples/enclaves/mutual_attestation_spec.v
@@ -1,0 +1,62 @@
+From iris.proofmode Require Import proofmode.
+From cap_machine Require Import rules logrel fundamental.
+From cap_machine Require Import proofmode.
+From cap_machine Require Import mutual_attestation_code.
+From cap_machine Require Import
+  mutual_attestation_code
+  mutual_attestation_A_spec
+  mutual_attestation_B_spec.
+
+
+Section mutual_attest_main.
+  Context {Σ:gFunctors} {ceriseg:ceriseG Σ} {sealsg : sealStoreG Σ}
+    {nainv: logrel_na_invs Σ} `{MP: MachineParameters}.
+  Context {MA: MutualAttestation}.
+
+
+  (* -------------------------------------------------- *)
+  (* ------------------- ENCLAVES --------------------- *)
+  (* -------------------------------------------------- *)
+
+  Lemma mutual_attest_contract :
+    custom_enclave_contract ma_enclaves_map.
+  Proof.
+    rewrite /custom_enclave_contract.
+    iIntros (I b e a v b' e' a' v' enclave_data ot ce
+      Hwf_cemap Hcode_ce Hot Hb' HIhash Hb He)
+      "(#Henclaves_inv & #Hma_inv & #HPenc & #HPsign)".
+    clear HIhash.
+    clear Hwf_cemap.
+    assert (e = (b ^+ (length (code ce) + 1))%a) as -> by solve_addr+He.
+
+    rewrite /ma_enclaves_map in Hcode_ce.
+    simplify_map_eq.
+
+    assert (I = hash_mutual_attest_A \/ I = hash_mutual_attest_B) as HI.
+    { rewrite lookup_insert_Some in Hcode_ce.
+      destruct Hcode_ce as [ [? _] | [_ Hcode_ce] ]; first auto.
+      rewrite lookup_insert_Some in Hcode_ce.
+      destruct Hcode_ce as [ [? _] | [_ Hcode_ce] ]; first auto.
+      done.
+    }
+    destruct HI ; simplify_map_eq.
+    - iApply ( mutual_attest_A_contract with "[]") ; last iFrame "#"; eauto.
+    - rewrite lookup_insert_ne // in Hcode_ce.
+      2:{ rewrite /hash_mutual_attest_A /hash_mutual_attest_B.
+          intro Hcontra.
+          apply hash_concat_inj' in Hcontra.
+          destruct Hcontra as [_ Hcontra].
+          rewrite /mutual_attest_enclave_A_code /mutual_attest_enclave_B_code in Hcontra.
+          by injection Hcontra.
+      }
+      simplify_map_eq.
+      iApply ( mutual_attest_B_contract with "[]") ; last iFrame "#"; eauto.
+  Admitted.
+
+  (* -------------------------------------------------- *)
+  (* ---------------------- MAIN ---------------------- *)
+  (* -------------------------------------------------- *)
+
+
+
+End mutual_attest_main.
